@prefix : <https://w3id.org/mint/ccut#> .
@prefix owl: <http://www.w3.org/2002/07/owl#> .
@prefix rdf: <http://www.w3.org/1999/02/22-rdf-syntax-ns#> .
@prefix xml: <http://www.w3.org/XML/1998/namespace> .
@prefix xsd: <http://www.w3.org/2001/XMLSchema#> .
@prefix rdfs: <http://www.w3.org/2000/01/rdf-schema#> .
@base <https://w3id.org/mint/ccut> .

<https://w3id.org/mint/ccut> rdf:type owl:Ontology ;
                              <http://purl.org/dc/terms/creator> "Arunkumar Rajendran" ,
                                                                 "Basel Shbita" ,
                                                                 "Jay Pujara" ;
                              <http://purl.org/dc/terms/license> <http://creativecommons.org/licenses/by/2.0/> ;
                              <http://purl.org/dc/terms/title> "Canonicalization Compound Unit Representation and Transformation Ontology" ;
                              <http://purl.org/vocab/vann/preferredNamespacePrefix> "ccut" ;
                              <http://purl.org/vocab/vann/preferredNamespaceUri> : ;
                              rdfs:comment "An ontology that describes units of measure for the MINT project" ;
                              owl:versionInfo "v1.0.0" .

#################################################################
#    Annotation properties
#################################################################

###  http://purl.org/dc/terms/creator
<http://purl.org/dc/terms/creator> rdf:type owl:AnnotationProperty .


###  http://purl.org/dc/terms/license
<http://purl.org/dc/terms/license> rdf:type owl:AnnotationProperty .


###  http://purl.org/dc/terms/title
<http://purl.org/dc/terms/title> rdf:type owl:AnnotationProperty .


###  http://purl.org/vocab/vann/preferredNamespacePrefix
<http://purl.org/vocab/vann/preferredNamespacePrefix> rdf:type owl:AnnotationProperty .


###  http://purl.org/vocab/vann/preferredNamespaceUri
<http://purl.org/vocab/vann/preferredNamespaceUri> rdf:type owl:AnnotationProperty .


#################################################################
#    Object Properties
#################################################################

###  https://w3id.org/mint/ccut#hasPart
:hasPart rdf:type owl:ObjectProperty ;
         rdfs:range :AtomicUnit ;
         rdfs:comment "Associates rdf:type compound unit with atomic units that compose it"@en ;
         rdfs:label "Has Part"@en .


###  https://w3id.org/mint/ccut#prefix
:prefix rdf:type owl:ObjectProperty ;
        rdfs:range <http://www.qudt.org/qudt/owl/1.0.0/qudt/#QuantityKind> ;
        rdfs:comment "Associates an SI (International System of Units) Prefix URI to some atomic unit"@en ;
        rdfs:label "Prefix"@en .


#################################################################
#    Data properties
#################################################################

###  https://w3id.org/mint/ccut#exponent
:exponent rdf:type owl:DatatypeProperty ;
          rdfs:range xsd:double ;
          rdfs:comment "Associates an exponent (dimension exponent) to some atomic unit"@en ;
          rdfs:label "Exponent"@en .


###  https://w3id.org/mint/ccut#hasDimension
:hasDimension rdf:type owl:DatatypeProperty ;
              rdfs:range xsd:string ;
              rdfs:comment "Associates an atomic or compound unit with rdf:type dimension string"@en ;
              rdfs:label "Has Dimension"@en .


###  https://w3id.org/mint/ccut#multiplier
:multiplier rdf:type owl:DatatypeProperty ;
            rdfs:range xsd:double ;
            rdfs:comment "Associates rdf:type multiplier (dimension prefix multiplier) to some atomic unit"@en ;
            rdfs:label "Multiplier"@en .


###  https://w3id.org/mint/ccut#prefixConversionMultiplier
:prefixConversionMultiplier rdf:type owl:DatatypeProperty ;
                            rdfs:range xsd:double ;
                            rdfs:comment "Associates an SI (International System of Units) Prefix Multiplier to some atomic unit"@en ;
                            rdfs:label "Prefix Conversion Multiplier"@en .


###  https://w3id.org/mint/ccut#prefixConversionOffset
:prefixConversionOffset rdf:type owl:DatatypeProperty ;
                        rdfs:range xsd:double ;
                        rdfs:comment "Associates an SI (International System of Units) Prefix Offset to some atomic unit"@en ;
                        rdfs:label "Prefix Conversion Offset"@en .


#################################################################
#    Classes
#################################################################

###  http://www.qudt.org/qudt/owl/1.0.0/qudt/#QuantityKind
<http://www.qudt.org/qudt/owl/1.0.0/qudt/#QuantityKind> rdf:type owl:Class .


###  https://w3id.org/mint/ccut#AtomicUnit
:AtomicUnit rdf:type owl:Class ;
            rdfs:comment "A class to represent rdf:type single unit symbol which may be modified by additional elements such as exponents or prefixes"@en ;
            rdfs:label "Atomic Unit"@en .


###  https://w3id.org/mint/ccut#CompoundUnit
:CompoundUnit rdf:type owl:Class ;
              rdfs:comment "A class to represent rdf:type complex unit that is composed from two or more atomic units with some relationship between them"@en ;
              rdfs:label "Compound Unit"@en .


###  Generated by the OWL API (version 5.1.9) https://github.com/owlcs/owlapi/
