@prefix rdf:   <http://www.w3.org/1999/02/22-rdf-syntax-ns#> .
@prefix rdfs:  <http://www.w3.org/2000/01/rdf-schema#> .
@prefix xml:   <http://www.w3.org/XML/1998/namespace> .
@prefix xsd:   <http://www.w3.org/2001/XMLSchema#> .
@prefix ccut:  <https://w3id.org/mint/ccut#> .
@prefix qudtp: <http://www.qudt.org/qudt/owl/1.0.0/qudt/Properties.html#> .
@prefix qudtu: <http://www.qudt.org/qudt/owl/1.0.0/unit/Instances.html#> .
@prefix qudt:  <http://www.qudt.org/qudt/owl/1.0.0/qudt/#> .
@prefix owl:   <http://www.w3.org/2002/07/owl#> .

<https://w3id.org/mint/ccut#> a owl:Ontology;
    owl:versionIRI <https://w3id.org/enigma/cohort/1.0.0> ;
    <http://purl.org/dc/terms/creator> "Basel Shbita",
                                       "Arunkumar Rajendran",
                                       "Jay Pujara" ;
    <http://purl.org/dc/terms/license> <http://creativecommons.org/licenses/by/2.0/> ;
    <http://purl.org/dc/terms/title> "Canonicalization Compound Unit Representation and Transformation Ontology" ;
    <http://purl.org/vocab/vann/preferredNamespacePrefix> "ccut" ;
    <http://purl.org/vocab/vann/preferredNamespaceUri> <https://w3id.org/mint/ccut#> ;
    rdfs:comment "An ontology that describes units of measure for the MINT project" ;
    owl:versionInfo "v1.0.0" .

ccut:atomicUnit a rdfs:Class ;
    rdfs:label                      "Atomic Unit"@en ;
    rdfs:comment                    "A class to represent a single unit symbol which may be modified by additional elements such as exponents or prefixes"@en ;
    qudtp:symbol                    xsd:string ;
    qudtp:conversionMultiplier      xsd:double ;
    qudtp:conversionOffset          xsd:double ;
    qudtp:quantityKind              qudt:QuantityKind ;
    ccut:prefix                     qudt:QuantityKind ;
    ccut:prefixConversionMultiplier xsd:double ;
    ccut:prefixConversionOffset     xsd:double ;
    ccut:exponent                   xsd:double ;
    ccut:multiplier                 xsd:double ;
    ccut:hasDimension               xsd:string .

ccut:compoundUnit a rdfs:Class ;
    rdfs:label                      "Compound Unit"@en ;
    rdfs:comment                    "A class to represent a complex unit that is composed from two or more atomic units with some relationship between them"@en ;
    qudtp:abbreviation              xsd:string ;
    ccut:hasPart                    ccut:atomicUnit ;
    ccut:hasDimension               xsd:string .

ccut:hasDimension a owl:DatatypeProperty ;
    rdfs:label      "Has Dimension"@en ;
    rdfs:comment    "Associates an atomic or compound unit with a dimension string"@en ;
    rdfs:range      xsd:string .

ccut:hasPart a owl:ObjectProperty ;
    rdfs:label      "Has Part"@en ;
    rdfs:comment    "Associates a compound unit with atomic units that compose it"@en ;
    rdfs:range      ccut:atomicUnit .

ccut:prefix a owl:ObjectProperty ;
    rdfs:label      "Prefix"@en ;
    rdfs:comment    "Associates an SI (International System of Units) Prefix URI to some atomic unit"@en ;
    rdfs:range      qudt:QuantityKind .

ccut:prefixConversionMultiplier a owl:DatatypeProperty ;
    rdfs:label      "Prefix Conversion Multiplier"@en ;
    rdfs:comment    "Associates an SI (International System of Units) Prefix Multiplier to some atomic unit"@en ;
    rdfs:range      xsd:double .

ccut:prefixConversionOffset a owl:DatatypeProperty ;
    rdfs:label      "Prefix Conversion Offset"@en ;
    rdfs:comment    "Associates an SI (International System of Units) Prefix Offset to some atomic unit"@en ;
    rdfs:range      xsd:double .

ccut:exponent a owl:DatatypeProperty ;
    rdfs:label      "Exponent"@en ;
    rdfs:comment    "Associates an exponent (dimension exponent) to some atomic unit"@en ;
    rdfs:range      xsd:double .

ccut:multiplier a owl:DatatypeProperty ;
    rdfs:label      "Multiplier"@en ;
    rdfs:comment    "Associates a multiplier (dimension prefix multiplier) to some atomic unit"@en ;
    rdfs:range      xsd:double .